# Question:

Given two $n-1$ degree polynomials: 

$$a_{n-1}x^{n-1} + a_{n-2}x^{n-2} + \cdots + a_{1}x^{1} + a_{0}x^{0}$$

$$b_{n-1}x^{n-1} + b_{n-2}x^{n-2} + \cdots + b_{1}x^{1} + b_{0}x^{0}$$

The multiplication product will be:

$$c_{2n-2}x^{2n-2} + c_{2n-3}x^{2n-3} + \cdots + c_{1}x^{1} + c_{0}x^{0}$$

where

$$c_{2n-2}x^{2n-2} = a_{n-1}b_{n-1}$$

$$c_{2n-3}x^{2n-3} = a_{n-1}b_{n-2} + a_{n-2}b_{n-1}$$

$$\vdots$$

$$c_{2} = a_{2}b_{0} + a_{1}b_{1} + a_{0}b_{2}$$

$$c_{1} = a_{1}b_{0} + a_{0]b_{1}$$

